Proofs/Proofs.lean
@@ -12,7 +12,8 @@ import Proofs.Popcount32
 import Proofs.Experiments.Summary1
 import Proofs.Experiments.MemoryAliasing
 import Proofs.Experiments.SHA512MemoryAliasing
-import Proofs.Experiments.Max
+import Proofs.Experiments.Max.MaxProgram
+import Proofs.Experiments.Max.MaxTandem
 import Proofs.Experiments.Abs.Abs
 import Proofs.Experiments.Abs.AbsVCG
 import Proofs.Experiments.Abs.AbsVCGTandem
